Function expansion verified using meta-extract

books/projects/smtlink/verified/expand-cp.lisp
@@ -1,10 +1,3 @@
-;; Copyright (C) 2015, University of British Columbia
-;; Written by Yan Peng (June 18th 2018)
-;;
-;; License: A 3-clause BSD license.
-;; See the LICENSE file distributed with ACL2
-;;
-
 (in-package "SMT")
 (include-book "std/util/bstar" :dir :system)
 (include-book "xdoc/top" :dir :system)
@@ -13,6 +6,7 @@
 (include-book "centaur/fty/basetypes" :dir :system)
 ;; for symbol-list-fix
 (include-book "centaur/fty/baselists" :dir :system)
+(include-book "centaur/misc/hons-extra" :dir :system)
 
 ;; Include SMT books
 (include-book "pseudo-lambda-lemmas")
@@ -27,657 +21,452 @@
 
 (include-book "clause-processors/just-expand" :dir :system)
 
-(defsection function-expansion
-  :parents (verified)
-  :short "Function expansion"
+(acl2::defevaluator-fast expev expev-lst
+                         ((if a b c) (equal a b) (not a)
+                          (cons a b) (binary-+ a b)
+                          (typespec-check ts x)
+                          (iff a b)
+                          (implies a b)
+                          (hint-please hint))
+                         :namedp t)
 
-  (defalist sym-nat-alist
-    :key-type symbol
-    :val-type natp
-    :pred sym-nat-alistp
-    :true-listp t)
+(acl2::def-ev-theoremp expev)
+(acl2::def-meta-extract expev expev-lst)
+(acl2::def-unify expev expev-alist)
 
+(defalist sym-nat-alist
+  :key-type symbol
+  :val-type natp
+  :pred sym-nat-alistp
+  :true-listp t)
+
+(local
+ (defthm consp-of-sym-nat-alist-fix
+   (implies (consp (sym-nat-alist-fix x)) (consp x))
+   :hints (("Goal" :in-theory (enable sym-nat-alist-fix))))
+ )
+
+(local
+ (defthm len-of-sym-nat-alist-fix-<
+   (> (1+ (len x)) (len (sym-nat-alist-fix x)))
+   :hints (("Goal" :in-theory (enable sym-nat-alist-fix))))
+ )
+
+(local
+ (defthm natp-of-cdar-sym-nat-alist-fix
+   (implies (consp (sym-nat-alist-fix x))
+            (natp (cdar (sym-nat-alist-fix x))))
+   :hints (("Goal" :in-theory (enable sym-nat-alist-fix))))
+ )
+
+(define update-fn-lvls ((fn symbolp) (fn-lvls sym-nat-alistp))
+  :returns (updated-fn-lvls sym-nat-alistp)
+  :measure (len fn-lvls)
+  :hints (("Goal" :in-theory (enable sym-nat-alist-fix)))
+  (b* ((fn (symbol-fix fn))
+       (fn-lvls (sym-nat-alist-fix fn-lvls))
+       ((unless (consp fn-lvls)) nil)
+       ((cons first rest) fn-lvls)
+       ((cons this-fn this-lvl) first)
+       ((unless (equal fn this-fn))
+        (cons (cons this-fn this-lvl)
+              (update-fn-lvls fn rest))))
+    (if (zp this-lvl)
+        (cons (cons this-fn 0) rest)
+      (cons (cons this-fn (1- this-lvl)) rest)))
+  ///
+  (more-returns
+   (updated-fn-lvls
+    (implies (and (symbolp fn)
+                  (sym-nat-alistp fn-lvls)
+                  (consp fn-lvls)
+                  (assoc-equal fn fn-lvls)
+                  (not (equal (cdr (assoc-equal fn fn-lvls)) 0)))
+             (< (cdr (assoc fn updated-fn-lvls))
+                (cdr (assoc fn fn-lvls))))
+    :name updated-fn-lvls-decrease))
+  )
+
+
+;; val-type can be a list of pseudo-termp
+;; This will give us two benefits: multiple facts and when it's nil,
+;; fact-finder fails to find a fact.
+(defalist fact-alist
+  :key-type pseudo-termp
+  :val-type pseudo-termp
+  :pred fact-alistp
+  :short "Value is the equivalence term about Key term."
+  :true-listp t)
+
+(defprod ex-args
+  :parents (function-expansion)
+  :short "Argument list for function expand"
+  ((fn-lvls sym-nat-alistp "Levels to expand each functions to."
+            :default nil)
+   (fn-lst func-alistp "List of function definitions to use for
+      function expansion." :default nil)
+   (facts fact-alistp "An alist of current learnt equivalence facts."
+          :default nil)
+   (fty-info fty-info-alist-p "FTY information." :default nil)
+   (wrld-fn-len natp "Number of function definitions in curent world."
+                :default 0)))
+
+(local
+ (defthm natp-of-sum-lvls-lemma
+   (implies (and (consp (sym-nat-alist-fix fn-lvls)) (natp x))
+            (natp (+ (cdr (car (sym-nat-alist-fix fn-lvls))) x)))
+   :hints (("Goal"
+            :in-theory (enable sym-nat-alist-fix)
+            :use ((:instance natp-of-cdar-sym-nat-alist-fix)))))
+ )
+
+(define sum-lvls ((fn-lvls sym-nat-alistp))
+  :returns (sum natp :hints (("Goal"
+                              :use ((:instance natp-of-sum-lvls-lemma
+                                               (x (sum-lvls (cdr (sym-nat-alist-fix fn-lvls)))))))))
+  :measure (len fn-lvls)
+  :hints (("Goal" :in-theory (enable sym-nat-alist-fix)))
+  (b* ((fn-lvls (sym-nat-alist-fix fn-lvls))
+       ((unless (consp fn-lvls)) 0)
+       ((cons first rest) fn-lvls)
+       ((cons & lvl) first))
+    (+ lvl (sum-lvls rest)))
+  ///
+  (defthm sum-lvls-decrease-after-update
+    (implies (and (symbolp fn)
+                  (sym-nat-alistp fn-lvls)
+                  (consp fn-lvls)
+                  (assoc-equal fn fn-lvls)
+                  (not (equal (cdr (assoc-equal fn fn-lvls)) 0)))
+             (< (sum-lvls (update-fn-lvls fn fn-lvls))
+                (sum-lvls fn-lvls)))
+    :hints (("Goal" :in-theory (enable update-fn-lvls)))))
+
+(encapsulate ()
+  (local (defthm alistp-of-pairlis$
+           (alistp (acl2::pairlis$ a b))))
+
+  (local (defthm pseudo-term-substp-of-pairlis$-for-pseudo-lambda
+           (implies (and (pseudo-term-listp x) (pseudo-lambdap y))
+                    (acl2::pseudo-term-substp (pairlis$ (lambda-formals y) x)))))
+
+  (define lambda-substitution ((fn-call pseudo-lambdap)
+                               (fn-actuals pseudo-term-listp))
+    :guard-hints (("Goal"
+                   :in-theory (e/d () (alistp-of-pairlis$
+                                       acl2::true-listp-when-symbol-listp))
+                   :use ((:instance acl2::true-listp-when-symbol-listp
+                                    (acl2::x (cadr fn-call)))
+                         (:instance alistp-of-pairlis$
+                                    (a (cadr fn-call))
+                                    (b fn-actuals)))))
+    :returns (subst-term pseudo-termp
+                         :hints (("Goal" :in-theory (e/d ()
+                                                         (pseudo-term-substp-of-pairlis$-for-pseudo-lambda
+                                                          acl2::return-type-of-substitute-into-term.xx))
+                                  :use ((:instance
+                                         pseudo-term-substp-of-pairlis$-for-pseudo-lambda
+                                         (x fn-actuals)
+                                         (y fn-call))
+                                        (:instance
+                                         acl2::return-type-of-substitute-into-term.xx
+                                         (x (lambda-body (pseudo-lambda-fix fn-call)))
+                                         (al (pairlis$ (lambda-formals
+                                                        (pseudo-lambda-fix fn-call))
+                                                       (pseudo-term-list-fix fn-actuals))))))))
+    (b* ((fn-call (pseudo-lambda-fix fn-call))
+         (fn-actuals (pseudo-term-list-fix fn-actuals))
+         (formals (lambda-formals fn-call))
+         (body (lambda-body fn-call)))
+      (acl2::substitute-into-term body (pairlis$ formals fn-actuals)))))
+
+(define function-substitution ((term pseudo-termp)
+                               state)
+  :returns (subst-term pseudo-termp
+                       :hints (("Goal"
+                                :in-theory (e/d ()
+                                                (pseudo-termp
+                                                 pseudo-term-listp
+                                                 acl2::return-type-of-substitute-into-term.xx
+                                                 acl2::return-type-of-simple-one-way-unify.a))
+                                :use ((:instance
+                                       acl2::return-type-of-simple-one-way-unify.a
+                                       (pat (cadr (acl2::meta-extract-formula-w
+                                                   (symbol-fix fn-call)
+                                                   (cdr (assoc-equal 'acl2::current-acl2-world
+                                                                     (nth 2 state))))))
+                                       (term (pseudo-term-fix term))
+                                       (alist nil))))))
+  (b* ((term (pseudo-term-fix term))
+       ((unless (and (not (acl2::variablep term))
+                     (not (acl2::fquotep term))
+                     (symbolp (car term))))
+        (prog2$
+         (er hard? 'expand-cp=>function-substitution "expand-cp: fn-call is nil
+                               or 'quote.")
+         nil))
+       ((cons fn-call &) term)
+       (formula (acl2::meta-extract-formula-w fn-call (w state)))
+       ((unless (pseudo-termp formula))
+        (prog2$
+         (er hard? 'expand-cp=>function-substitution "expand-cp: formula got by
+       meta-extract is not a pseudo-termp.")
+         nil))
+       ((mv ok lhs rhs)
+        (case-match formula
+          (('equal lhs rhs)
+           (mv t lhs rhs))
+          (& (mv nil nil nil))))
+       ((unless (and ok (pseudo-termp lhs)))
+        (prog2$ (er hard? 'expand-cp=>function-substitution "expand-cp: formula got by
+       meta-extract is not an equality.")
+                nil))
+       ((mv match-ok subst)
+        (acl2::simple-one-way-unify lhs term nil))
+       ((unless match-ok)
+        (prog2$
+         (er hard? 'expand-cp=>function-substitution "expand-cp:
+       simple-one-way-unify failed.")
+         nil)))
+    `(equal ,term ,(acl2::substitute-into-term rhs subst))))
+
+(encapsulate()
+(local (in-theory (e/d (function-substitution) (w))))
+
+(defthm function-substitution-correct
+  (implies (and (expev-meta-extract-global-facts)
+                (pseudo-termp term)
+                (alistp a)
+                (function-substitution term state))
+           (expev (function-substitution term state) a))
+  :hints (("Goal"
+           :in-theory (e/d ()
+                           (expev-meta-extract-formula))
+           :use ((:instance expev-meta-extract-formula
+                            (name (car term))
+                            (st state)
+                            (a (expev-alist (mv-nth 1
+                                                    (acl2::simple-one-way-unify
+                                                     (cadr (meta-extract-formula (car term) state))
+                                                     term nil))
+                                            a))))
+           ))
+  )
+)
+
+(encapsulate ()
   (local
-   (defthm consp-of-sym-nat-alist-fix
-     (implies (consp (sym-nat-alist-fix x)) (consp x))
-     :hints (("Goal" :in-theory (enable sym-nat-alist-fix))))
+   (defthm type-of-assoc-equal-of-sym-nat-alistp
+     (implies (and (sym-nat-alistp x)
+                   (symbolp y)
+                   (assoc-equal y x))
+              (and (symbolp (car (assoc-equal y x)))
+                   (natp (cdr (assoc-equal y x))))))
    )
 
-  (local
-   (defthm len-of-sym-nat-alist-fix-<
-     (> (1+ (len x)) (len (sym-nat-alist-fix x)))
-     :hints (("Goal" :in-theory (enable sym-nat-alist-fix))))
-   )
-
-  (local
-   (defthm natp-of-cdar-sym-nat-alist-fix
-     (implies (consp (sym-nat-alist-fix x))
-              (natp (cdar (sym-nat-alist-fix x))))
-     :hints (("Goal" :in-theory (enable sym-nat-alist-fix))))
-   )
-
-  (define update-fn-lvls ((fn symbolp) (fn-lvls sym-nat-alistp))
-    :returns (updated-fn-lvls sym-nat-alistp)
-    :measure (len fn-lvls)
-    :hints (("Goal" :in-theory (enable sym-nat-alist-fix)))
-    (b* ((fn (symbol-fix fn))
-         (fn-lvls (sym-nat-alist-fix fn-lvls))
-         ((unless (consp fn-lvls)) nil)
-         ((cons first rest) fn-lvls)
-         ((cons this-fn this-lvl) first)
-         ((unless (equal fn this-fn))
-          (cons (cons this-fn this-lvl)
-                (update-fn-lvls fn rest))))
-      (if (zp this-lvl)
-          (cons (cons this-fn 0) rest)
-        (cons (cons this-fn (1- this-lvl)) rest)))
+  (define fact-finder ((term pseudo-termp)
+                       (expand-args ex-args-p)
+                       state)
+    :guard (and (not (acl2::variablep term))
+                (not (acl2::fquotep term))
+                (symbolp (car term))
+                (not (assoc-equal term (ex-args->facts expand-args)))
+                (not (zp (ex-args->wrld-fn-len expand-args))))
+    :guard-hints (("Goal"
+                   :in-theory (e/d ()
+                                   (type-of-assoc-equal-of-sym-nat-alistp))
+                   :use ((:instance type-of-assoc-equal-of-sym-nat-alistp
+                                    (x (ex-args->fn-lvls expand-args))
+                                    (y (car term))))))
+    :returns (mv (new-term pseudo-termp)
+                 (new-args ex-args-p))
+    :short "Find the definition fact for @('term')"
+    :long "<p>Given a pseudo-termp @('term') that is not a @('variablep'), not
+a @('fquotep'), nor a @('pseudo-lambdap'), and that it doesn't exist in the
+list of facts learnt @('(ex-args->facts expand-args)'), we want to find the
+definition fact of that term.</p>
+"
+    (b* ((term (pseudo-term-fix term))
+         (expand-args (ex-args-fix expand-args))
+         ((ex-args a) expand-args)
+         ((cons fn &) term)
+         ;; There are three cases:
+         ;; 1. fn is a basic function (including fty functions) -- fn-lvls stays
+         ;; the same, nothing is expanded, no fact generated
+         ;; For 2 and 3, if fn-lvls is already 0, then do nothing; if fn-lvls is
+         ;; not 0, expand.
+         ;; 2. fn exists in user-defined fn-lvls -- fn-lvls decrease by 1, fn is
+         ;; expanded, one fact generated
+         ;; 3. otherwise, fn will be expanded once -- fn-lvls decrease by 1, fn
+         ;; is expanded, one fact generated
+         (basic-function (member-equal fn *SMT-basics*))
+         (flex? (fncall-of-flextype fn a.fty-info))
+         ((if (or basic-function flex?)) (mv nil a))
+         (lvl (assoc-equal fn a.fn-lvls))
+         (user-defined (assoc-equal fn a.fn-lst))
+         ((if (and lvl (zp (cdr lvl)) user-defined)) (mv nil a))
+         ((if (and lvl (zp (cdr lvl)) (null user-defined)))
+          (prog2$ (er hard? 'expand-cp=>fact-finder "Possibly
+                       encountered recursive functions that are not user-defined.")
+                  (mv nil a)))
+         (fact (function-substitution term state))
+         ((if (null fact)) (mv nil a))
+         ((if lvl)
+          (mv fact
+              (make-ex-args :fn-lvls (update-fn-lvls fn a.fn-lvls)
+                            :fn-lst a.fn-lst
+                            :facts (acons term fact a.facts)
+                            :fty-info a.fty-info
+                            :wrld-fn-len a.wrld-fn-len))))
+      ;; if not in fn-lvls
+      (mv fact
+          (make-ex-args :fn-lst a.fn-lst
+                        :fn-lvls (cons `(,fn . 0) a.fn-lvls)
+                        :facts (acons term fact a.facts)
+                        :fty-info a.fty-info
+                        :wrld-fn-len (1- a.wrld-fn-len))))
     ///
     (more-returns
-     (updated-fn-lvls
-      (implies (and (symbolp fn)
-                    (sym-nat-alistp fn-lvls)
-                    (consp fn-lvls)
-                    (assoc-equal fn fn-lvls)
-                    (not (equal (cdr (assoc-equal fn fn-lvls)) 0)))
-               (< (cdr (assoc fn updated-fn-lvls))
-                  (cdr (assoc fn fn-lvls))))
-      :name updated-fn-lvls-decrease))
+     (new-args
+      (implies
+       (and (pseudo-termp term)
+            (ex-args-p expand-args)
+            (symbolp (car term))
+            new-term
+            (assoc-equal (car term)
+                         (ex-args->fn-lvls expand-args)))
+       (and (< (sum-lvls (ex-args->fn-lvls new-args))
+               (sum-lvls (ex-args->fn-lvls expand-args)))
+            (equal (ex-args->wrld-fn-len new-args)
+                   (ex-args->wrld-fn-len expand-args))))
+      :hints (("Goal"
+               :in-theory (e/d ()
+                               (sum-lvls-decrease-after-update))
+               :use ((:instance sum-lvls-decrease-after-update
+                                (fn (car term))
+                                (fn-lvls (ex-args->fn-lvls expand-args))))))
+      :name fact-finder-decrease-1)
+     (new-args
+      (implies
+       (and (pseudo-termp term)
+            (ex-args-p expand-args)
+            (symbolp (car term))
+            (not (zp (ex-args->wrld-fn-len expand-args)))
+            new-term
+            (not (assoc-equal (car term)
+                              (ex-args->fn-lvls expand-args))))
+       (< (ex-args->wrld-fn-len new-args)
+          (ex-args->wrld-fn-len expand-args)))
+      :name fact-finder-decrease-2)
+     (new-args
+      (implies (not new-term)
+               (and (equal (ex-args->wrld-fn-len new-args)
+                           (ex-args->wrld-fn-len expand-args))
+                    (equal (sum-lvls (ex-args->fn-lvls new-args))
+                           (sum-lvls (ex-args->fn-lvls expand-args)))))
+      :name fact-finder-same-3)
+     )
     )
+  )
 
+(include-book "ordinals/lexicographic-ordering" :dir :system)
+(set-state-ok t)
 
-  (defprod ex-args
-    :parents (function-expansion)
-    :short "Argument list for function expand"
-    :long "<p>@('Ex-args') stores the list of arguments passed into the
-    function @(see expand). We design this product type so that we don't have a
-    long list of arguments to write down every time there's a recursive call.
-    This document describes what each argument is about and more specifically,
-    why they exist necessarily. This document comes out because every time when
-    I read the @(see expand) function, I get confused and lost track about why I
-    designed such a argument in the first place.</p>
+(defines expand
+  :well-founded-relation l<
+  :flag-local nil
+  :verify-guards nil
+  :flag-defthm-macro defthm-expand
+  :measure-debug t
 
-    <p>@('Term-lst') is easy, it stores the list of terms to be expanded.
-    Recursively generated new terms are stored in this argument and gets used
-    in recursive calls. Using a list of terms allows us to use a single
-    recursive function instead of @(see mutual-recursion), even though every
-    time we call this function, we really just have one term to expand.</p>
-
-    <p>@('Fn-lst') stores a list of function definitions for use of expansion.
-    This list comes from the @(see smtlink-hint) stored in function stub @(see
-    smt-hint). Such a list initially comes from user inputs to @(see Smtlink).
-    So it can be, for example, some functions that the user wants to get
-    expanded specially.</p>
-
-    <p>@('Fn-lvls') stores a list of maximum number of times each function
-    needs to be expanded. This list doesn't take into account of functions that
-    are not specified by the user, which should oftenly be the case. In that
-    case, those functions will be expanded just once and a pair will be stored
-    into @('fn-lvls') indicating this function has already been expanded. This
-    is done by storing a level of 0 for such a function.</p>
-
-    <p>@('Wrld-fn-len') is the hardest to explain. But given some thought, I
-    found it to be necessary to have this argument. @('wrld-fn-len') represents
-    the length of current ACL2 @(see world), meaning the number of definitions
-    in total (might be more than that, I'm not completely sure about what the
-    @(see world) is composed of). This argument helps prove termination of
-    function @(see expand). See @(see expand-measure) for a discussion about
-    the measure function for proving termimation.</p>
-
-    <p>@('Expand-lst') stores all functions that are expanded in @(see expand).
-    This list gets used later for generating the @(':in-theory') hint for
-    proving that the expanded term implies the original unexpanded term.</p>"
-
-    ((term-lst pseudo-term-listp "List of terms to be expanded. The function
-    finishes when all of them are expanded to given level."
-               :default nil)
-     (fn-lst func-alistp "List of function definitions to use for
-      function expansion." :default nil)
-     (fn-lvls sym-nat-alistp "Levels to expand each functions to." :default
-              nil)
-     (wrld-fn-len natp "Number of function definitions in curent world."
-                  :default 0)
-     (expand-lst pseudo-term-alistp "An alist of expanded function symbols
-    associated with their function call" :default nil)))
-
-  (defprod ex-outs
-    :parents (function-expansion)
-    :short "Outputs for function expand"
-    ((expanded-term-lst pseudo-term-listp "List of expanded terms." :default nil)
-     (expanded-fn-lst pseudo-term-alistp "List of expanded function calls,
-    needed for expand hint for proving G' implies G theorem." :default nil)))
-
-  (local
-   (defthm natp-of-sum-lvls-lemma
-     (implies (and (consp (sym-nat-alist-fix fn-lvls)) (natp x))
-              (natp (+ (cdr (car (sym-nat-alist-fix fn-lvls))) x)))
-     :hints (("Goal"
-              :in-theory (enable sym-nat-alist-fix)
-              :use ((:instance natp-of-cdar-sym-nat-alist-fix)))))
-   )
-
-  (define sum-lvls ((fn-lvls sym-nat-alistp))
-    :returns (sum natp :hints (("Goal"
-                                :use ((:instance natp-of-sum-lvls-lemma
-                                                 (x (sum-lvls (cdr (sym-nat-alist-fix fn-lvls)))))))))
-    :measure (len fn-lvls)
-    :hints (("Goal" :in-theory (enable sym-nat-alist-fix)))
-    (b* ((fn-lvls (sym-nat-alist-fix fn-lvls))
-         ((unless (consp fn-lvls)) 0)
-         ((cons first rest) fn-lvls)
-         ((cons & lvl) first))
-      (+ lvl (sum-lvls rest)))
-    ///
-    (defthm sum-lvls-decrease-after-update
-      (implies (and (symbolp fn)
-                    (sym-nat-alistp fn-lvls)
-                    (consp fn-lvls)
-                    (assoc-equal fn fn-lvls)
-                    (not (equal (cdr (assoc-equal fn fn-lvls)) 0)))
-               (< (sum-lvls (update-fn-lvls fn fn-lvls))
-                  (sum-lvls fn-lvls)))
-      :hints (("Goal" :in-theory (enable update-fn-lvls)))))
-
-  (define expand-measure ((expand-args ex-args-p))
-    :returns (m nat-listp)
-    :parents (function-expansion)
-    :short "@(see acl2::Measure) function for proving termination of function
-    @(see expand)."
-
-    :long "<p>The measure is using the lexicographical order (see @(see
-    mutual-recursion)), using a list of three arguments, where the priority
-    goes from the first argument to the second, and then to the third.</p>
-
-    <p>The first argument is @('wrld-fn-len') which appears in @(see ex-args).
-    It is necessary for decreasing the measure when we are expanding a function
-    that is not in @('fn-lst') (see @(see ex-args)). The second argument is a
-    summation of @('fn-lvls') which also appears in @(see ex-args). This list
-    remembers how many levels are left for each function. Since functions not
-    in @('fn-lst') are added to @('fn-lvls') with 0 level, this argument
-    doesn't decrease in that case. This is why it's necessary to have the first
-    argument @('wrld-fn-len'). The third argument is the @(see acl2-count) of
-    current @('term-lst') (also see @(see ex-args)). This argument decreases
-    every time the recursive function @('expand') goes into expand the @(see
-    cdr) of @('term-lst').</p>"
-
-    (b* ((expand-args (ex-args-fix expand-args))
+  (define expand-list ((term-lst pseudo-term-listp)
+                       (expand-args ex-args-p)
+                       state)
+    :returns (fact-alst fact-alistp)
+    :measure (list (ex-args->wrld-fn-len expand-args)
+                   (sum-lvls (ex-args->fn-lvls expand-args))
+                   (acl2-count (pseudo-term-list-fix term-lst)))
+    (b* ((term-lst (pseudo-term-list-fix term-lst))
+         (expand-args (ex-args-fix expand-args))
          ((ex-args a) expand-args)
-         (lvl-sum (sum-lvls a.fn-lvls)))
-      (list a.wrld-fn-len lvl-sum (acl2-count a.term-lst))))
+         ((unless (consp term-lst)) a.facts)
+         ((cons first rest) term-lst)
+         (facts-first (expand first a state)))
+      (expand-list rest (change-ex-args a :facts facts-first) state)))
 
-  (encapsulate ()
-    (local (defthm lemma-1
-             (implies (ex-args-p x)
-                      (pseudo-term-listp (ex-args->term-lst x)))))
-
-    (local (defthm lemma-2
-             (implies (and (pseudo-term-listp y) (consp y))
-                      (pseudo-termp (car y)))))
-
-    (local (defthm lemma-3
-             (implies (and (pseudo-termp z) (consp z) (not (equal (car z) 'quote)))
-                      (pseudo-term-listp (cdr z)))))
-
-    (defthm pseudo-term-list-of-cdar-of-ex-args->term-lst
-      (implies (and (ex-args-p expand-args)
-                    (consp (ex-args->term-lst expand-args))
-                    (consp (car (ex-args->term-lst expand-args)))
-                    (not (equal (caar (ex-args->term-lst expand-args)) 'quote)))
-               (pseudo-term-listp (cdar (ex-args->term-lst expand-args)))))
-
-    (local (defthm lemma-4
-             (implies (and (pseudo-term-listp y) (consp y))
-                      (pseudo-term-listp (cdr y)))))
-
-    (defthm pseudo-term-listp-of-cdr-of-ex-args->term-lst
-      (implies (and (ex-args-p expand-args)
-                    (consp (ex-args->term-lst expand-args)))
-               (pseudo-term-listp (cdr (ex-args->term-lst expand-args)))))
-
-    (local (defthm lemma-5
-             (implies (and (pseudo-term-listp y) (consp y) (not (consp (car y))))
-                      (symbolp (car y)))))
-
-    (defthm symbolp-of-car-of-ex-args->term-lst
-      (implies (and (ex-args-p expand-args)
-                    (consp (ex-args->term-lst expand-args))
-                    (not (consp (car (ex-args->term-lst expand-args)))))
-               (symbolp (car (ex-args->term-lst expand-args)))))
-
-    (defthm pseudo-termp-of-car-of-ex-args->term-lst
-      (implies (and (ex-args-p expand-args)
-                    (consp (ex-args->term-lst expand-args)))
-               (pseudo-termp (car (ex-args->term-lst expand-args))))
-      :hints (("Goal" :in-theory (enable pseudo-termp))))
-
-    (defthm len-equal-of-formals-of-pseudo-lambdap-and-actuals-of-pseudo-termp
-      (implies (and (ex-args-p expand-args)
-                    (pseudo-termp (car (ex-args->term-lst expand-args)))
-                    (pseudo-lambdap (car (car (ex-args->term-lst expand-args)))))
-               (equal (len (cadr (car (car (ex-args->term-lst expand-args)))))
-                      (len (cdr (car (ex-args->term-lst expand-args))))))
-      :hints (("Goal" :in-theory (e/d (pseudo-termp pseudo-lambdap)
-                                      (ACL2::FOLD-CONSTS-IN-+
-                                       ACL2::PSEUDO-TERMP-CAR)))))
-
-    (local (defthm lemma-6
-             (implies (and (pseudo-termp x) (not (symbolp x)) (not (pseudo-lambdap (car x))))
-                      (symbolp (car x)))
-             :hints (("Goal" :in-theory (enable pseudo-termp pseudo-lambdap)))))
-
-    (defthm symbolp-of-caar-of-ex-args->term-lst
-      (implies (and (ex-args-p expand-args)
-                    (consp (ex-args->term-lst expand-args))
-                    (not (symbolp (car (ex-args->term-lst expand-args))))
-                    (not (pseudo-lambdap (car (car (ex-args->term-lst expand-args))))))
-               (symbolp (car (car (ex-args->term-lst expand-args))))))
-
-    (local (defthm lemma-7
-             (implies (and (pseudo-termp x) (consp x) (equal (car x) 'quote))
-                      (and (not (cddr x)) (consp (cdr x))))))
-
-    (defthm not-cddr-of-car-of-pseudo-term-list-fix-of-expand-args->term-lst
-      (implies (and (consp (ex-args->term-lst expand-args))
-                    (consp (car (ex-args->term-lst expand-args)))
-                    (not (symbolp (car (ex-args->term-lst expand-args))))
-                    (equal (car (car (ex-args->term-lst expand-args))) 'quote))
-               (not (cddr (car (ex-args->term-lst expand-args))))))
-
-    (defthm consp-cdr-of-car-of-pseudo-term-list-fix-of-expand-args->term-lst
-      (implies (and (consp (ex-args->term-lst expand-args))
-                    (consp (car (ex-args->term-lst expand-args)))
-                    (not (symbolp (car (ex-args->term-lst expand-args))))
-                    (equal (car (car (ex-args->term-lst expand-args))) 'quote))
-               (consp (cdr (car (ex-args->term-lst expand-args))))))
-
-    (defthm pseudo-term-listp-of-pseudo-lambdap-of-cdar-ex-args->term-lst
-      (implies (and (ex-args-p expand-args)
-                    (consp (ex-args->term-lst expand-args))
-                    (consp (car (ex-args->term-lst expand-args)))
-                    (not (equal (caar (ex-args->term-lst expand-args)) 'quote)))
-               (pseudo-term-listp (cdar (ex-args->term-lst expand-args)))))
-    )
-
-  (encapsulate ()
-    (local (in-theory (enable pseudo-lambdap)))
-
-    (defthm symbol-listp-of-formals-of-pseudo-lambdap
-      (implies (pseudo-lambdap x) (symbol-listp (cadr x))))
-
-    (defthm pseudo-termp-of-body-of-pseudo-lambdap
-      (implies (pseudo-lambdap x) (pseudo-termp (caddr x))))
-
-    (defthm consp-of-pseudo-lambdap
-      (implies (pseudo-lambdap x) (consp x)))
-
-    (defthm consp-of-cdr-of-pseudo-lambdap
-      (implies (pseudo-lambdap x) (consp (cdr x))))
-
-    (defthm consp-of-cddr-of-pseudo-lambdap
-      (implies (pseudo-lambdap x) (consp (cddr x))))
-
-    (defthm not-stringp-of-cadr-of-pseudo-lambdap
-      (implies (pseudo-lambdap x) (not (stringp (cadr x)))))
-    )
-
-  (encapsulate ()
-    (local (defthm lemma-1
-             (implies (ex-args-p x) (sym-nat-alistp (ex-args->fn-lvls x)))))
-
-    (local (defthm lemma-2
-             (implies (and (sym-nat-alistp y) (assoc-equal foo y))
-                      (natp (cdr (assoc-equal foo y))))))
-
-    (local (defthm lemma-3
-             (implies (and (sym-nat-alistp y) (assoc-equal foo y))
-                      (consp (assoc-equal foo y)))))
-
-    (local (defthm natp-of-cdr-of-assoc-equal-of-ex-args->fn-lvls-of-ex-args-p
-             (implies (and (ex-args-p x) (assoc-equal foo (ex-args->fn-lvls x)))
-                      (natp (cdr (assoc-equal foo (ex-args->fn-lvls x)))))))
-
-    (defthm integerp-of-cdr-of-assoc-equal-of-ex-args->fn-lvls-of-ex-args-p
-      (implies (and (ex-args-p x) (assoc-equal foo (ex-args->fn-lvls x)))
-               (integerp (cdr (assoc-equal foo (ex-args->fn-lvls x)))))
-      :hints(("Goal" :use ((:instance
-                            natp-of-cdr-of-assoc-equal-of-ex-args->fn-lvls-of-ex-args-p (x x))))))
-
-    (defthm non-neg-of-cdr-of-assoc-equal-of-ex-args->fn-lvls-of-ex-args-p
-      (implies (and (ex-args-p x) (assoc-equal foo (ex-args->fn-lvls x)))
-               (<= 0 (cdr (assoc-equal foo (ex-args->fn-lvls x)))))
-      :hints(("Goal" :use ((:instance
-                            natp-of-cdr-of-assoc-equal-of-ex-args->fn-lvls-of-ex-args-p (x x))))))
-
-    (defthm consp-of-assoc-equal-of-ex-args->fn-lvls-of-ex-args-p
-      (implies (and (ex-args-p x) (assoc-equal foo (ex-args->fn-lvls x)))
-               (consp (assoc-equal foo (ex-args->fn-lvls x)))))
-
-    (defthm last-<=
-      (<= (acl2-count (last x))
-          (acl2-count x)))
-
-    (defthm last-pseudo-term-list-is-pseudo-term-list
-      (implies (pseudo-term-listp x)
-               (pseudo-term-listp (last x))))
-    )
-
-  (local (in-theory (enable expand-measure)))
-  (encapsulate
-    ()
-    (set-well-founded-relation l<)
-    (local (in-theory (e/d
-                       ()
-                       (ACL2::PSEUDO-LAMBDAP-OF-CAR-WHEN-PSEUDO-TERMP
-                        ACL2::SUBSETP-CONS-2
-                        CONSP-OF-SYM-NAT-ALIST-FIX
-                        DEFAULT-CDR
-                        SYM-NAT-ALISTP-OF-CDR-WHEN-SYM-NAT-ALISTP
-                        NTH
-                        TRUE-LISTP
-                        ACL2::PSEUDO-LAMBDAP-OF-CAR-WHEN-PSEUDO-LAMBDA-LISTP
-                        ACL2::PSEUDO-LAMBDA-LISTP-OF-CDR-WHEN-PSEUDO-LAMBDA-LISTP
-                        ACL2::PSEUDO-TERMP-CDR-ASSOC-EQUAL
-                        SYM-NAT-ALISTP-WHEN-NOT-CONSP
-                        ACL2::SUBSETP-CAR-MEMBER
-                        STRIP-CDRS
-                        (:TYPE-PRESCRIPTION SYM-NAT-ALIST-FIX$INLINE)
-                        ACL2::SUBSETP-WHEN-ATOM-RIGHT
-                        RATIONAL-LISTP
-                        INTEGER-LISTP
-                        ATOM
-                        ACL2::SYMBOL-LISTP-WHEN-NOT-CONSP
-                        ACL2::PSEUDO-LAMBDAP-WHEN-MEMBER-EQUAL-OF-PSEUDO-LAMBDA-LISTP
-                        ACL2::SYMBOL-LISTP-CDR-ASSOC-EQUAL
-                        ACL2::SYMBOL-LIST-LISTP
-                        ACL2::RATIONALP-OF-CAR-WHEN-RATIONAL-LISTP
-                        ACL2::INTEGERP-OF-CAR-WHEN-INTEGER-LISTP
-                        CONSP-WHEN-MEMBER-EQUAL-OF-SYM-NAT-ALISTP
-                        ACL2::CONSP-WHEN-MEMBER-EQUAL-OF-SYMBOL-SYMBOL-ALISTP
-                        ACL2::PSEUDO-LAMBDAP-OF-NTH-WHEN-PSEUDO-LAMBDA-LISTP
-                        ACL2::PSEUDO-LAMBDA-LISTP-WHEN-NOT-CONSP
-                        ACL2::SUBSETP-WHEN-ATOM-LEFT))))
-
-    ;; Q FOR YAN:
-    ;; 1. merge expand-args->fn-lst and expand-args->fn-lvls
-    ;; 2. change update-fn-lvls function so that old items are not deleted and update the measure function
-    ;; 3. clean the code in a more structured way - treat lambdas in another function
-    ;; 4. clean up the above encapsulated theorems, maybe in another file
-    (define expand ((expand-args ex-args-p) (fty-info fty-info-alist-p) state)
-      :parents (function-expansion)
-      :returns (expanded-result ex-outs-p)
-      :measure (expand-measure expand-args)
-      :verify-guards nil
-      :hints
-      (("Goal"
-        :in-theory (e/d ()
-                        (last-<=
-                         sum-lvls-decrease-after-update))
-        :use ((:instance last-<=
-                         (x (cdr (car (ex-args->term-lst expand-args)))))
-              (:instance sum-lvls-decrease-after-update
-                         (fn (car (car (ex-args->term-lst expand-args))))
-                         (fn-lvls (ex-args->fn-lvls expand-args))))))
-      (b* ((expand-args (ex-args-fix expand-args))
-           (fty-info (fty-info-alist-fix fty-info))
-           ;; This binds expand-args to a, so that we can call a.term-lst ...
-           ((ex-args a) expand-args)
-           ((unless (consp a.term-lst))
-            (make-ex-outs :expanded-term-lst nil :expanded-fn-lst a.expand-lst))
-           ((cons term rest) a.term-lst)
-           ;; If first term is a symbolp, return the symbol
-           ;; then recurse on the rest of the list
-           ((if (symbolp term))
-            (b* ((rest-res (expand (change-ex-args a :term-lst rest) fty-info
-                                   state))
-                 ((ex-outs o) rest-res))
-              (make-ex-outs :expanded-term-lst (cons term o.expanded-term-lst)
-                            :expanded-fn-lst o.expanded-fn-lst)))
-           ((if (equal (car term) 'quote))
-            (b* ((rest-res (expand (change-ex-args a :term-lst rest) fty-info
-                                   state))
-                 ((ex-outs o) rest-res))
-              (make-ex-outs :expanded-term-lst (cons term o.expanded-term-lst)
-                            :expanded-fn-lst o.expanded-fn-lst)))
-           ;; The first term is now a function call:
-           ;; Cons the function call and function actuals out of term
-           ((cons fn-call fn-actuals) term)
-
-           ;; If fn-call is a pseudo-lambdap
-           ((if (pseudo-lambdap fn-call))
-            (b* ((lambda-formals (lambda-formals fn-call))
-                 (body-res
-                  (expand (change-ex-args a
-                                          :term-lst (list (lambda-body
-                                                           fn-call)))
-                          fty-info state))
-                 ((ex-outs b) body-res)
-                 (lambda-body (car b.expanded-term-lst))
-                 (actuals-res
-                  (expand (change-ex-args a
-                                          :term-lst fn-actuals
-                                          :expand-lst b.expanded-fn-lst)
-                          fty-info state))
-                 ((ex-outs ac) actuals-res)
-                 (lambda-actuals ac.expanded-term-lst)
-                 ((unless (mbt (equal (len lambda-formals) (len lambda-actuals))))
-                  (make-ex-outs :expanded-term-lst a.term-lst :expanded-fn-lst a.expand-lst))
-                 (lambda-fn `((lambda ,lambda-formals ,lambda-body) ,@lambda-actuals))
-                 (rest-res
-                  (expand (change-ex-args a
-                                          :term-lst rest
-                                          :expand-lst ac.expanded-fn-lst)
-                          fty-info state))
-                 ((ex-outs r) rest-res))
-              (make-ex-outs :expanded-term-lst (cons lambda-fn r.expanded-term-lst)
-                            :expanded-fn-lst r.expanded-fn-lst)))
-
-           ;; If fn-call is neither a lambda expression nor a function call
-           ((unless (mbt (symbolp fn-call)))
-            (make-ex-outs :expanded-term-lst a.term-lst :expanded-fn-lst a.expand-lst))
-           ;; Try finding function call from fn-lst
-           (fn (hons-get fn-call a.fn-lst))
-           ;; If fn-call doesn't exist in fn-lst, it can be a basic function,
-           ;; in that case we don't do anything with it.
-           ;; Otherwise it can be a function that's forgotten to be added to fn-lst.
-           ;; We are going to expand all function like this for one level.
-           ;; If the function is basic or has already been expanded once.
-           ((unless fn)
-            (b* (((unless (function-symbolp fn-call (w state)))
-                  (prog2$
-                   (er hard? 'SMT-goal-generator=>expand "Should be a function call: ~q0" fn-call)
-                   (make-ex-outs :expanded-term-lst a.term-lst :expanded-fn-lst a.expand-lst)))
-                 (basic-function (member-equal fn-call *SMT-basics*))
-                 (flex? (fncall-of-flextype fn-call fty-info))
-                 (lvl-item (assoc-equal fn-call a.fn-lvls))
-                 (extract-res (meta-extract-formula fn-call state))
-                 ((if (equal fn-call 'return-last))
-                  (b* ((actuals-res
-                        (expand (change-ex-args a :term-lst (last fn-actuals))
-                                fty-info state))
-                       ((ex-outs ac) actuals-res)
-                       (rest-res
-                        (expand (change-ex-args a :term-lst rest
-                                                :expand-lst ac.expanded-fn-lst)
-                                fty-info state))
-                       ((ex-outs r) rest-res))
-                    (make-ex-outs
-                     :expanded-term-lst (cons
-                                         (car ac.expanded-term-lst)
-                                         r.expanded-term-lst)
-                     :expanded-fn-lst r.expanded-fn-lst)))
-                 ((if (or basic-function flex?
-                          (<= a.wrld-fn-len 0) (and lvl-item (zp (cdr lvl-item)))
-                          (equal extract-res ''t)))
-                  (b* ((actuals-res
-                        (expand (change-ex-args a :term-lst fn-actuals)
-                                fty-info state))
-                       ((ex-outs ac) actuals-res)
-                       (rest-res
-                        (expand (change-ex-args a :term-lst rest
-                                                :expand-lst ac.expanded-fn-lst)
-                                fty-info state))
-                       ((ex-outs r) rest-res))
-                    (make-ex-outs :expanded-term-lst (cons (cons fn-call ac.expanded-term-lst) r.expanded-term-lst)
-
-                                  :expanded-fn-lst r.expanded-fn-lst)))
-                 (formals (formals fn-call (w state)))
-                 ((unless (symbol-listp formals))
-                  (prog2$
-                   (er hard? 'SMT-goal-generator=>expand "formals get a list that's not a symbol-listp for ~q0, the formals are ~q1" fn-call formals)
-                   (make-ex-outs :expanded-term-lst a.term-lst :expanded-fn-lst a.expand-lst)))
-                 ((unless (true-listp extract-res))
-                  (prog2$
-                   (er hard? 'SMT-goal-generator=>expand "meta-extract-formula returning a non-true-listp for ~q0The extracted result is ~q1" fn-call extract-res)
-                   (make-ex-outs :expanded-term-lst a.term-lst :expanded-fn-lst a.expand-lst)))
-                 (body (nth 2 extract-res))
-                 ((unless (pseudo-termp body))
-                  (prog2$
-                   (er hard? 'SMT-goal-generator=>expand "meta-extract-formula returning a non-pseudo-term for ~q0The body is ~q1" fn-call body)
-                   (make-ex-outs :expanded-term-lst a.term-lst :expanded-fn-lst a.expand-lst)))
-                 ;; (- (cw "SMT-goal-generator=>Expanding ... ~q0" fn-call))
-                 ;; Adding function symbol into expand-lst
-                 (updated-expand-lst
-                  (if (assoc-equal term a.expand-lst)
-                      a.expand-lst (cons `(,term . ,term) a.expand-lst)))
-                 (body-res
-                  (expand (change-ex-args a
-                                          :term-lst (list body)
-                                          :fn-lvls (cons `(,fn-call . 0) a.fn-lvls)
-                                          :wrld-fn-len (1- a.wrld-fn-len)
-                                          :expand-lst updated-expand-lst)
-                          fty-info state))
-                 ((ex-outs b) body-res)
-                 ;; Expand function
-                 (expanded-lambda-body (car b.expanded-term-lst))
-                 (expanded-lambda `(lambda ,formals ,expanded-lambda-body))
-                 (actuals-res
-                  (expand (change-ex-args a :term-lst fn-actuals
-                                          :expand-lst b.expanded-fn-lst)
-                          fty-info state))
-                 ((ex-outs ac) actuals-res)
-                 (expanded-term-list ac.expanded-term-lst)
-                 ((unless (equal (len formals) (len expanded-term-list)))
-                  (prog2$
-                   (er hard? 'SMT-goal-generator=>expand "You called your function with the wrong number of actuals: ~q0" term)
-                   (make-ex-outs :expanded-term-lst a.term-lst :expanded-fn-lst ac.expanded-fn-lst)) )
-                 (rest-res
-                  (expand (change-ex-args a :term-lst rest
-                                          :expand-lst ac.expanded-fn-lst)
-                          fty-info state))
-                 ((ex-outs r) rest-res))
-              (make-ex-outs :expanded-term-lst (cons `(,expanded-lambda ,@expanded-term-list) r.expanded-term-lst)
-                            :expanded-fn-lst r.expanded-fn-lst)))
-
-           ;; Now fn is a function in fn-lst
-           ;; If fn-call is already expanded to level 0, don't expand.
-           (lvl-item (assoc-equal fn-call a.fn-lvls))
-           ((unless lvl-item)
-            (prog2$
-             (er hard? 'SMT-goal-generator=>expand "Function ~q0 exists in the definition list but not in the levels list?" fn-call)
-             (make-ex-outs :expanded-term-lst a.term-lst :expanded-fn-lst a.expand-lst)) )
-           ((if (zp (cdr lvl-item)))
-            (b* ((actuals-res
-                  (expand (change-ex-args a :term-lst fn-actuals)
-                          fty-info state))
-                 ((ex-outs ac) actuals-res)
-                 (rest-res
-                  (expand (change-ex-args a :term-lst rest
-                                          :expand-lst ac.expanded-fn-lst)
-                          fty-info state))
-                 ((ex-outs r) rest-res))
-              (make-ex-outs :expanded-term-lst (cons (cons fn-call ac.expanded-term-lst) r.expanded-term-lst)
-
-                            :expanded-fn-lst r.expanded-fn-lst)))
-
-           ;; If fn-call is not expanded to level 0, still can expand.
-           (new-fn-lvls (update-fn-lvls fn-call a.fn-lvls))
-           ((func f) (cdr fn))
-           (extract-res (meta-extract-formula fn-call state))
-           ((unless (true-listp extract-res))
-            (prog2$
-             (er hard? 'SMT-goal-generator=>expand "meta-extract-formula returning a non-true-listp for ~q0The extracted result is ~q1" fn-call extract-res)
-             (make-ex-outs :expanded-term-lst a.term-lst :expanded-fn-lst a.expand-lst)))
-           (body (nth 2 extract-res))
-           ((unless (pseudo-termp body))
-            (prog2$
-             (er hard? 'SMT-goal-generator=>expand "meta-extract-formula returning a non-pseudo-term for ~q0The body is ~q1" fn-call body)
-             (make-ex-outs :expanded-term-lst a.term-lst :expanded-fn-lst a.expand-lst)))
-           ;; (- (cw "SMT-goal-generator=>Expanding ... ~q0" fn-call))
-           (updated-expand-lst
-            (if (assoc-equal term a.expand-lst)
-                a.expand-lst (cons `(,term . ,term) a.expand-lst)))
-           (formals f.flattened-formals)
-           (body-res
-            (expand (change-ex-args a :term-lst (list body)
-                                    :fn-lvls new-fn-lvls
-                                    :expand-lst updated-expand-lst)
-                    fty-info state))
-           ((ex-outs b) body-res)
-           (expanded-lambda-body (car b.expanded-term-lst))
-           (expanded-lambda `(lambda ,formals ,expanded-lambda-body))
-           (actuals-res
-            (expand (change-ex-args a :term-lst fn-actuals
-                                    :expand-lst b.expanded-fn-lst)
-                    fty-info state))
-           ((ex-outs ac) actuals-res)
-           (expanded-term-list ac.expanded-term-lst)
-           ((unless (equal (len formals) (len expanded-term-list)))
-            (prog2$
-             (er hard? 'SMT-goal-generator=>expand "You called your function with the wrong number of actuals: ~q0" term)
-             (make-ex-outs :expanded-term-lst a.term-lst :expanded-fn-lst ac.expanded-fn-lst)))
-           (rest-res
-            (expand (change-ex-args a :term-lst rest
-                                    :expand-lst ac.expanded-fn-lst)
-                    fty-info state))
-           ((ex-outs r) rest-res))
-        (make-ex-outs :expanded-term-lst (cons `(,expanded-lambda ,@expanded-term-list) r.expanded-term-lst)
-                      :expanded-fn-lst r.expanded-fn-lst))
-      ///
-      (more-returns
-       (expanded-result (implies (ex-args-p expand-args)
-                                 (pseudo-term-alistp
-                                  (ex-outs->expanded-fn-lst expanded-result)))
-                        :name pseudo-term-alistp-of-expand)
-       (expanded-result (implies (ex-args-p expand-args)
-                                 (pseudo-term-listp
-                                  (ex-outs->expanded-term-lst expanded-result)))
-                        :name pseudo-term-listp-of-expand)
-       (expanded-result (implies (ex-args-p expand-args)
-                                 (pseudo-termp
-                                  (car (ex-outs->expanded-term-lst expanded-result))))
-                        :name pseudo-termp-of-car-of-expand)
-       (expanded-result (implies (ex-args-p expand-args)
-                                 (equal (len (ex-outs->expanded-term-lst expanded-result))
-                                        (len (ex-args->term-lst expand-args))))
-                        :name len-of-expand)
-       )
-      )
-    )
-
-  (verify-guards expand
+  (define expand ((term pseudo-termp)
+                  (expand-args ex-args-p)
+                  state)
+    :returns (fact-alst fact-alistp)
+    :measure (list (ex-args->wrld-fn-len expand-args)
+                   (sum-lvls (ex-args->fn-lvls expand-args))
+                   (acl2-count (pseudo-term-fix term)))
     :hints (("Goal"
-             :in-theory (e/d
-                         ()
-                         (NTH
-                          FGETPROP
-                          TRUE-LISTP
-                          DEFAULT-CDR
-                          ASSOC-EQUAL
-                          ACL2::SUBSETP-CONS-2
-                          ACL2::O-P-O-INFP-CAR
-                          CONSP-OF-SYM-NAT-ALIST-FIX
-                          ACL2::SYMBOL-LISTP-WHEN-NOT-CONSP
-                          ACL2::PSEUDO-LAMBDA-LISTP-WHEN-NOT-CONSP
-                          ACL2::PSEUDO-LAMBDAP-OF-CAR-WHEN-PSEUDO-TERMP
-                          CONSP-WHEN-MEMBER-EQUAL-OF-SYM-NAT-ALISTP
-                          SYM-NAT-ALISTP-OF-CDR-WHEN-SYM-NAT-ALISTP
-                          ACL2::PSEUDO-LAMBDAP-OF-NTH-WHEN-PSEUDO-LAMBDA-LISTP
-                          ACL2::PSEUDO-LAMBDA-LISTP-OF-CDR-WHEN-PSEUDO-LAMBDA-LISTP
-                          ACL2::PSEUDO-LAMBDAP-OF-CAR-WHEN-PSEUDO-LAMBDA-LISTP
-                          ACL2::CONSP-WHEN-MEMBER-EQUAL-OF-SYMBOL-SYMBOL-ALISTP
-                          ACL2::PSEUDO-LAMBDAP-WHEN-MEMBER-EQUAL-OF-PSEUDO-LAMBDA-LISTP))
-             :use ((:instance pseudo-term-listp-of-pseudo-lambdap-of-cdar-ex-args->term-lst)
-                   (:instance symbolp-of-caar-of-ex-args->term-lst)))))
+             :in-theory (e/d ()
+                             (fact-finder-decrease-1
+                              fact-finder-decrease-2
+                              fact-finder-same-3))
+             :use ((:instance fact-finder-decrease-1
+                              (term (pseudo-term-fix term))
+                              (expand-args (ex-args-fix expand-args)))
+                   (:instance fact-finder-decrease-2
+                              (term (pseudo-term-fix term))
+                              (expand-args (ex-args-fix expand-args)))
+                   (:instance fact-finder-same-3
+                              (term (pseudo-term-fix term))
+                              (expand-args (ex-args-fix expand-args)))
+                   )))
+    (b* ((term (pseudo-term-fix term))
+         (expand-args (ex-args-fix expand-args))
+         ((ex-args a) expand-args)
+         ((if (zp a.wrld-fn-len)) a.facts)
+         ;; If first term is a symbolp or is quoted, return the current facts
+         ((if (or (acl2::variablep term) (acl2::fquotep term))) a.facts)
+         ;; The first term is now a function call:
+         ;; Cons the function call and function actuals out of term
+         ((cons fn-call fn-actuals) term)
+         ;; If fn-call is a pseudo-lambdap, substitute unbounded variables in the
+         ;; lambda and recurse to expand the substituted term.
+         ;; To ensure termination, wrld-fn-len needs to decrease, this means
+         ;; wrld-fn-len should include term size so that it's large enough.
+         ((if (pseudo-lambdap fn-call))
+          (expand (lambda-substitution fn-call fn-actuals)
+                  (change-ex-args a :wrld-fn-len (1- a.wrld-fn-len))
+                  state))
+         ;; If fn-call is neither a lambda expression nor a function call
+         ((unless (mbt (symbolp fn-call))) nil)
 
+         ;; -----------------------------------------------------------
+         ;; Now the term is a function call, we first test if term already exists
+         ;; in facts alist.
+         (exists? (assoc-equal term a.facts))
+         ;; I can skip the whole subtree because if such a term already exists in
+         ;; facts, then it's subterms, subsubterms ... must also exist in the
+         ;; facts. This is because we are doing a depth first travesal.
+         ((if exists?) a.facts)
+         ((mv new-term new-args) (fact-finder term a state))
+         ;; new-term being nil meaning there's no fact to prove
+         ((unless new-term)
+          (expand-list fn-actuals new-args state))
+         (body-fact (expand new-term new-args state))
+         (actuals-fact
+          (expand-list fn-actuals
+                       (change-ex-args new-args :facts body-fact)
+                       state)))
+      actuals-fact))
+  )
+
+(encapsulate ()
+  (local
+   (defthm symbolp-of-fn-call-of-pseudo-termp
+     (implies (and (pseudo-termp x)
+                   (consp x)
+                   (not (acl2::fquotep x))
+                   (not (pseudo-lambdap (car x))))
+              (symbolp (car x)))
+     :hints (("Goal" :in-theory (enable pseudo-lambdap)))))
+
+  (verify-guards expand)
   )
 
 (define initialize-fn-lvls ((fn-lst func-alistp))
@@ -716,30 +505,62 @@
        (fty-types (reverse ordered-acc)))
     (change-smtlink-hint h :fty-types fty-types)))
 
-;; -----------------------------------------------------------------
-;;       Define evaluators
+(define compose-goal ((cl pseudo-term-listp)
+                      (to-be-learnt pseudo-term-listp)
+                      state)
+  :returns (new-goal pseudo-term-listp)
+  :measure (len (pseudo-term-list-fix to-be-learnt))
+  (b* ((cl (pseudo-term-list-fix cl))
+       (to-be-learnt (pseudo-term-list-fix to-be-learnt))
+       ((unless (consp to-be-learnt)) cl)
+       ((cons first-fact rest-facts) to-be-learnt)
+       ((unless (and (not (acl2::variablep first-fact))
+                     (not (acl2::fquotep first-fact))
+                     (symbolp (car first-fact))))
+        cl)
+       (learnt-fact (function-substitution first-fact state))
+       ((if (null learnt-fact)) cl))
+    `((not ,learnt-fact)
+      ,@(compose-goal cl rest-facts state))))
 
-(defevaluator ev-expand-cp ev-lst-expand-cp
-  ((not x) (if x y z) (hint-please hint)))
+(encapsulate ()
+(local (in-theory (e/d (compose-goal) ())))
 
-(def-join-thms ev-expand-cp)
+(defthm compose-goal-correct
+  (implies (and (expev-meta-extract-global-facts)
+                (pseudo-term-listp clause)
+                (alistp a)
+                (expev (disjoin
+                        (compose-goal clause to-be-learnt state))
+                       a))
+           (expev (disjoin clause) a))
+  :hints (("Goal"
+           :expand (compose-goal clause to-be-learnt state)
+           :use
+           ((:instance function-substitution-correct
+                       (term (car (pseudo-term-list-fix to-be-learnt)))
+                       (a a)
+                       (state state)))
+           ))
+  )
+)
 
-;; -----------------------------------------------------------------
-
-;; Define the function expansion clause processor
-;; Expanded-G
-;; Expanded-G => G
+(encapsulate ()
+  (local
+   (defthm pseudo-term-listp-of-strip-cars-of-fact-alistp
+     (implies (fact-alistp x)
+              (pseudo-term-listp (strip-cars x)))))
 
 (define expand-cp-helper ((cl pseudo-term-listp)
-                          (smtlink-hint smtlink-hint-p)
+                          (smtlink-hint t)
                           state)
-  :returns (new-hint smtlink-hint-p)
-  :guard-debug t
-  (b* ((cl (pseudo-term-list-fix cl))
-       (smtlink-hint (smtlink-hint-fix smtlink-hint))
+  :returns (subgoal-lst pseudo-term-list-listp)
+  (b* (((unless (pseudo-term-listp cl)) nil)
+       ((unless (smtlink-hint-p smtlink-hint))
+        (list cl))
        ;; generate all fty related stuff
        (flextypes-table (table-alist 'fty::flextypes-table (w state)))
-       ((unless (alistp flextypes-table)) smtlink-hint)
+       ((unless (alistp flextypes-table)) (list cl))
        (h1 (generate-fty-info-alist smtlink-hint flextypes-table))
        (h2 (generate-fty-types-top h1 flextypes-table))
        ((smtlink-hint h) h2)
@@ -749,62 +570,41 @@
        (wrld-fn-len h.wrld-fn-len)
        (G (disjoin cl))
        ;; Do function expansion
-       (expand-result
-        (with-fast-alist fn-lst (expand (make-ex-args
-                                         :term-lst (list G)
-                                         :fn-lst fn-lst
-                                         :fn-lvls fn-lvls
-                                         :wrld-fn-len wrld-fn-len)
-                                        h.fty-info state)))
-       ((ex-outs e) expand-result)
-       (expanded-G (car e.expanded-term-lst))
-       ;; generate expand hint
-       (fncall-lst (strip-cars e.expanded-fn-lst))
-       ((unless (alistp fncall-lst))
-        (prog2$
-         (er hard? 'expand=>expand-cp "Function call list should be an alistp: ~
-                   ~q0" fncall-lst)
-         h))
-       (expand-hint (remove-duplicates-equal (strip-cars fncall-lst)))
-       (hint-with-fn-expand (treat-in-theory-hint expand-hint h.main-hint))
-       (expanded-clause-w/-hint (make-hint-pair :thm expanded-G
-                                                :hints hint-with-fn-expand)))
-    (change-smtlink-hint h
-                         :expanded-clause-w/-hint expanded-clause-w/-hint)))
-
-(define expand-cp-fn ((cl pseudo-term-listp)
-                      (smtlink-hint t))
-  :returns (subgoal-lst pseudo-term-list-listp)
-  (b* (((unless (pseudo-term-listp cl)) nil)
-       ((unless (smtlink-hint-p smtlink-hint))
-        (list cl))
-       (G (disjoin cl))
-       (hinted-expanded-G
-        (smtlink-hint->expanded-clause-w/-hint smtlink-hint))
-       (expanded-G (hint-pair->thm hinted-expanded-G))
-       (main-hint (hint-pair->hints hinted-expanded-G))
-       ;; generate first clause
+       (facts nil)
+       (to-be-learnt
+        (with-fast-alists (facts fn-lvls fn-lst)
+          (expand G (make-ex-args
+                     :fn-lvls fn-lvls
+                     :fn-lst fn-lst
+                     :facts facts
+                     :fty-info h.fty-info
+                     :wrld-fn-len wrld-fn-len)
+                  state)))
+       (expanded-goal (compose-goal cl (strip-cars to-be-learnt) state))
        (next-cp (cdr (assoc-equal 'expand *SMT-architecture*)))
        ((if (null next-cp)) (list cl))
        (the-hint
         `(:clause-processor (,next-cp clause ',smtlink-hint)))
-       (cl0 `((hint-please ',the-hint) ,expanded-G))
-       ;; generate-second clause
-       (cl1 `((hint-please ',main-hint) (not ,expanded-G) ,G))
-       )
-    `(,cl0 ,cl1)))
+       (hinted-goal `((hint-please ',the-hint) ,@expanded-goal)))
+    (list hinted-goal)))
+)
 
-(defmacro expand-cp (clause hint)
-  `(expand-cp-fn clause (expand-cp-helper ,clause ,hint state)))
+(define expand-cp ((cl pseudo-term-listp)
+                   (hints t)
+                   state)
+  (b* ((expanded-clause (expand-cp-helper cl hints state)))
+    (value expanded-clause)))
 
-;; proving correctness of the expansion clause processor
-(local (in-theory (enable expand-cp-fn)))
+(local (in-theory (enable expand-cp expand-cp-helper)))
 
 (defthm correctness-of-expand-cp
-  (implies (and (pseudo-term-listp cl)
-                (alistp b)
-                (ev-expand-cp
-                 (conjoin-clauses (expand-cp-fn cl smtlink-hint))
-                 b))
-           (ev-expand-cp (disjoin cl) b))
+  (implies (and (expev-meta-extract-global-facts)
+                (pseudo-term-listp clause)
+                (alistp a)
+                (expev
+                 (conjoin-clauses
+                  (acl2::clauses-result
+                   (expand-cp clause hints state)))
+                 a))
+           (expev (disjoin clause) a))
   :rule-classes :clause-processor)
