books/projects/smtlink/examples/examples.lisp
@@ -31,7 +31,11 @@
                   (<=  (x^2-y^2 x y) 1))
              (< y (- (* 3 (- x (/ 17 8)) (- x (/ 17 8))) 3)))
     :hints(("Goal"
-            :smtlink nil)))
+            :smtlink
+            (:functions ((x^2-y^2 :formals ((x real/rationalp)
+                                            (y real/rationalp))
+                                  :returns ((f real/rationalp))
+                                  :level 1))))))
   )
 
 (deftutorial Example-1
